Weidenbach_Book/IsaSAT/IsaSAT_Backtrack_LLVM.thy
@@ -1,6 +1,6 @@
 theory IsaSAT_Backtrack_LLVM
   imports IsaSAT_Backtrack IsaSAT_VMTF_LLVM IsaSAT_Lookup_Conflict_LLVM
-    IsaSAT_Rephase_LLVM
+    IsaSAT_Rephase_LLVM IsaSAT_LBD_LLVM
 begin
 
 lemma isa_empty_conflict_and_extract_clause_heur_alt_def:
@@ -148,6 +148,7 @@ sepref_def propagate_bt_wl_D_fast_codeXX
 lemma extract_shorter_conflict_list_heur_st_alt_def:
     \<open>extract_shorter_conflict_list_heur_st = (\<lambda>(M, N, (bD), Q', W', vm, clvls, cach, lbd, outl,
        stats, ccont, vdom). do {
+     lbd \<leftarrow> mark_lbd_from_list_heur M outl lbd;
      let D =  the_lookup_conflict bD;
      ASSERT(fst M \<noteq> []);
      let K = lit_of_last_trail_pol M;
