Weidenbach_Book/IsaSAT/IsaSAT_LBD_LLVM.thy
@@ -2,7 +2,8 @@ theory IsaSAT_LBD_LLVM
   imports IsaSAT_LBD IsaSAT_Setup_LLVM
 begin
 
-sepref_register mark_lbd_from_clause_heur get_level_pol
+sepref_register mark_lbd_from_clause_heur get_level_pol mark_lbd_from_list_heur
+  mark_lbd_from_conflict
 
 sepref_def mark_lbd_from_clause_heur_impl
   is \<open>uncurry3 mark_lbd_from_clause_heur\<close>
@@ -13,12 +14,30 @@ sepref_def mark_lbd_from_clause_heur_impl
   by sepref
 
 sepref_def calculate_LBD_heur_st_impl
-  is \<open>uncurry calculate_LBD_heur_st\<close>
-  :: \<open>isasat_bounded_assn\<^sup>d *\<^sub>a sint64_nat_assn\<^sup>k \<rightarrow>\<^sub>a isasat_bounded_assn\<close>
+  is \<open>uncurry3 calculate_LBD_heur_st\<close>
+  :: \<open>trail_pol_fast_assn\<^sup>k *\<^sub>a arena_fast_assn\<^sup>d *\<^sub>a lbd_assn\<^sup>d *\<^sub>a sint64_nat_assn\<^sup>k \<rightarrow>\<^sub>a
+     arena_fast_assn \<times>\<^sub>a lbd_assn\<close>
   supply [[goals_limit=1]]
   unfolding calculate_LBD_heur_st_def isasat_bounded_assn_def
     fold_tuple_optimizations
   apply (annot_unat_const \<open>TYPE(32)\<close>)
+  by sepref
+
+sepref_def mark_lbd_from_list_heur_impl
+  is \<open>uncurry2 mark_lbd_from_list_heur\<close>
+  :: \<open>trail_pol_fast_assn\<^sup>k *\<^sub>a out_learned_assn\<^sup>k *\<^sub>a lbd_assn\<^sup>d \<rightarrow>\<^sub>a lbd_assn\<close>
+  supply [[goals_limit=1]]
+  unfolding mark_lbd_from_list_heur_def nfoldli_upt_by_while
+  apply (rewrite at \<open>_ = \<hole>\<close> unat_const_fold[where 'a=32])
+  apply (annot_snat_const \<open>TYPE(64)\<close>)
+  by sepref
+
+sepref_def mark_lbd_from_conflict_impl
+  is \<open>mark_lbd_from_conflict\<close>
+  :: \<open>isasat_bounded_assn\<^sup>d \<rightarrow>\<^sub>a isasat_bounded_assn\<close>
+  supply [[goals_limit=1]]
+  unfolding mark_lbd_from_conflict_def isasat_bounded_assn_def
+    fold_tuple_optimizations
   by sepref
 
 end
